PP_CakeML.sig
@@ -7,29 +7,17 @@ sig
     type decl = AST.decl
     type tydec = AADL.tydec
     type tmdec = AADL.tmdec
+    type outdec = AADL.outdec
     type pretty = PolyML.pretty
     type contig = ByteContig.contig
-    type tyenvs = (id -> ty) * (qid -> ty) *  (qid -> ty)
+    type tyenvs = (id -> ty) * (qid -> ty) * (qid -> ty)
     type port = string * ty * string * string
     type ivar = string * ty * exp
-    type guar = string * string * exp
 
     val pp_cake_ty : int -> string -> ty -> pretty
     val pp_cake_exp : int -> string -> tyenvs -> exp -> pretty
     val pp_tydec : int -> string -> AADL.tydec -> pretty
     val pp_tmdec : int -> string -> tyenvs -> AADL.tmdec -> pretty
-
-    val mk_tyE         : AADL.pkg list -> qid -> ty option
-    val mk_constE      : AADL.pkg list -> string -> ty option
-    val mk_recd_projns : tydec list -> tmdec list
-    val empty_varE     : id -> ty option
-    val assocFn        : (''a * 'b) list -> ''a -> 'b option
-    val transRval      : ((qid -> ty option) * (id -> ty option)) * (id -> ty option)
-                          -> exp -> exp
-    val tydec_to_ty    : tydec -> ty
-    val contig_to_exp  : (string * contig) list -> contig -> exp
-    val AppExp         : exp list -> exp
-    val listLit        : exp list -> exp
 
     val pp_api : string *
                  (string * int) list *      (* inport bufs *)
@@ -38,9 +26,11 @@ sig
                  string -> pretty
 
     val pp_parser_struct
-      : string * port list * (qid * contig) list * tmdec list -> pretty
+       : string * port list * (qid * contig) list * tmdec list -> pretty
 
-    val pp_defs_struct : tyenvs -> string * tydec list * tmdec list -> pretty
+    val pp_defs_struct
+       : tyenvs -> string * tydec list * tmdec list -> pretty
 
-    val pp_gadget_struct : tyenvs -> string * port list * ivar list * outdec list -> pretty
+    val pp_gadget_struct
+       : tyenvs -> string * port list * ivar list * outdec list -> pretty
 end
