agree/aprogScript.sml
@@ -21,17 +21,18 @@
 (*                                                                           *)
 (*   type valEnv = string |-> value                                          *)
 (*                                                                           *)
-(* We also separate the environment into inputs, outputs, and state vars.    *)
+(* We now separate the environment into inputs, outputs, and state vars.     *)
 (* An evaluation step of a component is a map from an (input,state) env pair *)
 (* to a (state,output) pair, where the envs are valEnvs.                     *)
 (*                                                                           *)
-(*   stateStep : comp -> (valEnv * valEnv) -> (valEnv * valEnv)              *)
+(*   stateStep : comp -> (valEnv # valEnv) -> (valEnv # valEnv)              *)
 (*                                                                           *)
 (* At this point, the environments can be made explicit as parameters to a   *)
 (* function definition.                                                      *)
 (*                                                                           *)
 (*   fnStep : input-tuple * state-tuple -> state-tuple * output-tuple        *)
 (*                                                                           *)
+(* where tuple elements are values.                                          *)
 (*---------------------------------------------------------------------------*)
 
 open HolKernel Parse boolLib bossLib BasicProvers
@@ -76,6 +77,20 @@ Definition arithprog_def:
       guarantees  := []
       |>
 End
+
+overload_on ("/\\",``AndExpr``);
+overload_on ("COND",``BoolCondExpr``);
+overload_on ("=",``EqExpr``);
+overload_on ("pre",``PreExpr``);
+overload_on ("pre",``BoolPreExpr``);
+overload_on ("<=",``LeqExpr``);
+overload_on ("<",``LessExpr``);
+overload_on ("+",``AddExpr``);
+overload_on ("-",``SubExpr``);
+overload_on ("=",``BoolStmt``);
+overload_on ("=",``IntStmt``);
+overload_on ("-->",``FbyExpr``);
+
 
 val th0 = EVAL“(strmSteps E arithprog 0 ' "out") 0”
 val th1 = EVAL“(strmSteps E arithprog 1 ' "out") 1”
@@ -126,9 +141,9 @@ QED
 (*---------------------------------------------------------------------------*)
 
 
-Definition iter_arithprog_def:
-  iter_arithprog =
-    <| inports  := ["input"];
+Definition itprog_def:
+  itprog =
+    <| inports  := ["input"; "isInit"];
        var_defs :=
           [IntStmt "N" (FbyExpr (IntLit 0)
                                 (AddExpr (PreExpr (IntVar "N")) (IntLit 1)));
@@ -148,13 +163,13 @@ Definition iter_arithprog_def:
       |>
 End
 
-val th0 = EVAL“(strmSteps E iter_arithprog 0 ' "out") 0”
-val th1 = EVAL“(strmSteps E iter_arithprog 1 ' "out") 1”
-val th2 = EVAL“(strmSteps E iter_arithprog 2 ' "out") 2”
-val th3 = EVAL“(strmSteps E iter_arithprog 3 ' "out") 3”
-val th4 = EVAL“(strmSteps E iter_arithprog 4 ' "out") 4”
-val th5 = EVAL“(strmSteps E iter_arithprog 5 ' "out") 5”
-val th6 = EVAL“(strmSteps E iter_arithprog 6 ' "out") 6”
+val th0 = EVAL“(strmSteps E itprog 0 ' "out") 0”
+val th1 = EVAL“(strmSteps E itprog 1 ' "out") 1”
+val th2 = EVAL“(strmSteps E itprog 2 ' "out") 2”
+val th3 = EVAL“(strmSteps E itprog 3 ' "out") 3”
+val th4 = EVAL“(strmSteps E itprog 4 ' "out") 4”
+val th5 = EVAL“(strmSteps E itprog 5 ' "out") 5”
+val th6 = EVAL“(strmSteps E itprog 6 ' "out") 6”
 ;
 
 (*--------------------------------------------------------------------------*)
@@ -162,63 +177,176 @@ val th6 = EVAL“(strmSteps E iter_arithprog 6 ' "out") 6”
 (* "pre"s squashed out.                                                     *)
 (*--------------------------------------------------------------------------*)
 
-val iter_arithprog_ap =
-   EVAL “strmStep E iter_arithprog t ' "ap" t” |> SIMP_RULE (srw_ss()) [];
+val itprog_ap =
+   EVAL “strmStep E itprog t ' "ap" t” |> SIMP_RULE (srw_ss()) [];
 
-val iter_arithprog_out =
-   EVAL “strmStep E iter_arithprog t ' "out" t” |> SIMP_RULE (srw_ss()) [];
+val itprog_out =
+   EVAL “strmStep E itprog t ' "out" t” |> SIMP_RULE (srw_ss()) [];
 
 
-Theorem iter_arithprog_Eq_out_ap[local] :
- ∀t E. strmStep E iter_arithprog t ' "out" t = strmStep E iter_arithprog t ' "ap" t
+Theorem itprog_Eq_out_ap[local] :
+ ∀t E. strmStep E itprog t ' "out" t = strmStep E itprog t ' "ap" t
 Proof
-  rw [iter_arithprog_ap,iter_arithprog_out]
+  rw [itprog_ap,itprog_out]
 QED
 
-Theorem iter_arithprog_Vars_Eq[local] :
- ∀t E. strmSteps E iter_arithprog t ' "out" t = strmSteps E iter_arithprog t ' "ap" t
+Theorem itprog_Vars_Eq[local] :
+ ∀t E. strmSteps E itprog t ' "out" t = strmSteps E itprog t ' "ap" t
 Proof
-  Induct >> rw [strmSteps_def,iter_arithprog_ap,iter_arithprog_out]
+  Induct >> rw [strmSteps_def,itprog_ap,itprog_out]
 QED
 
-(* Probably needs to be generalized to include more vars.
 Theorem equiv1:
-  ∀E t. strmSteps E arithprog t ' "out" t = strmSteps E iter_arithprog t ' "out" t
+  ∀E t. strmSteps E arithprog t ' "out" t = strmSteps E itprog t ' "out" t
 Proof
-  simp [arithprog_Vars_Eq, iter_arithprog_Vars_Eq]
+  simp [arithprog_Vars_Eq, itprog_Vars_Eq]
   >> Induct_on ‘t’
-  >-  (EVAL_TAC >> rw[])
-  >-  (EVAL_TAC >> rw[GSYM arithprog_def, GSYM iter_arithprog_def]
-       >- (‘t = 0n’ by decide_tac >> rw [] >> EVAL_TAC >> rw[])
-       >-
-QED
- *)
+  >> cheat
 
-(* Relates a stream step to a state step.
-    - Think about whether it needs to relate strmSteps and stateSteps
-    - stateIn is taken at time t and so is stateOut. Probably needs to be t and SUC t
-    -
+(* >-  (EVAL_TAC >> rw[])
+   >-  (EVAL_TAC >> rw[GSYM arithprog_def, GSYM itprog_def]
+        >- (‘t = 0n’ by decide_tac >> rw [] >> EVAL_TAC >> rw[])
+        >-
+*)
+QED
+
+
+val expand_Supports = CONV_TAC (STRIP_QUANT_CONV (LAND_CONV (PATH_CONV "lr" EVAL)));
+
+val itprog_inports = (EVAL THENC SIMP_CONV (srw_ss()) []) “itprog.inports” ;
+val itprog_var_defs = (EVAL THENC SIMP_CONV (srw_ss()) []) “itprog.var_defs” ;
+val itprog_out_defs = (EVAL THENC SIMP_CONV (srw_ss()) []) “itprog.out_defs” ;
+val itprog_varDecs = (EVAL THENC SIMP_CONV (srw_ss()) []) “varDecs itprog” ;
+
+
+Theorem strmIndex_DRESTRICT :
+ ∀E P t. strmIndex (DRESTRICT E P) t = DRESTRICT (strmIndex E t) P
+Proof
+ rw [strmIndex_def,fmap_EXT,FMAP_MAP2_def,FUN_FMAP_DEF,DRESTRICT_DEF]
+QED
+
+Triviality lem :
+  "input" IN FDOM E ∧
+  "isInit" IN FDOM E ∧
+  isInit_Stream (E ' "isInit")
+   ⇒
+  DRESTRICT (strmIndex E t) {"input";"isInit"}
+   =
+  (FEMPTY |++ [("input", E ' "input" t) ;
+               ("isInit", BoolValue (t=0))])
+Proof
+  rw [fmap_EXT,DRESTRICT_DEF,strmIndex_def,EXTENSION,IN_INTER,
+      FMAP_MAP2_def,FUN_FMAP_DEF,isInit_Stream_def,FUPDATE_LIST_THM]
+  >- metis_tac[]
+  >- EVAL_TAC
+  >- (EVAL_TAC >> rw[])
+QED
+
+Definition initState_def:
+  initState = (FEMPTY |++
+    [("N",    IntValue ARB);
+     ("ap",   BoolValue ARB);
+     ("in2",  IntValue ARB);
+     ("in1",  IntValue ARB)])
+End
+
+Theorem equiv2_step:
+  Supports E itprog ∧
+  0 < t ∧
+  isInit_Stream (E ' "isInit") ∧
+  inE = strmIndex (input_of itprog E) t ∧
+  stE = state_of itprog (strmIndex E (t-1)) ∧
+  E' = strmStep E itprog t
+  ⇒
+  stateStep itprog (inE, stE)
+   =
+  (state_of itprog (strmIndex E' t),
+   output_of itprog (strmIndex E' t))
+Proof
+  expand_Supports
+  >> simp[]
+  >> EVAL_TAC
+  >> rw [FUPDATE_LIST_THM,FUNION_FUPDATE_1,FUNION_FUPDATE_2,DRESTRICT_FUPDATE,FDOM_DRESTRICT]
+  >- (qpat_x_assum ‘bool_of _’ mp_tac
+       >> CONV_TAC (LAND_CONV (SIMP_CONV (srw_ss()) [FUNION_DEF]))
+       >> ASM_REWRITE_TAC[]
+       >> rw [DRESTRICT_DEF,EXTENSION,IN_INTER,FUN_FMAP_DEF]
+       >> fs[bool_of_def])
+
+  >- (qpat_x_assum ‘bool_of _’ mp_tac
+       >> CONV_TAC (LAND_CONV (SIMP_CONV (srw_ss()) [FUNION_DEF]))
+       >> ASM_REWRITE_TAC[]
+       >> rw [DRESTRICT_DEF,EXTENSION,IN_INTER,FUN_FMAP_DEF]
+       >> fs[bool_of_def])
+
+  >- (rw[fmap_EXT,FDOM_DRESTRICT,SUBSET_DEF]
+      >> rw [DRESTRICT_DEF,EXTENSION,IN_INTER,FUN_FMAP_DEF]
+      >- rw [EQ_IMP_THM]
+      >> rw[FUNION_DEF,DRESTRICT_DEF,EXTENSION,IN_INTER,FUN_FMAP_DEF,combinTheory.APPLY_UPDATE_THM]
+      >> rw [FAPPLY_FUPDATE_THM])
+
+  >- (rw[fmap_EXT,FDOM_DRESTRICT,SUBSET_DEF]
+      >> rw [DRESTRICT_DEF,EXTENSION,IN_INTER,FUN_FMAP_DEF]
+      >- rw [EQ_IMP_THM]
+      >> rw[FUNION_DEF,DRESTRICT_DEF,EXTENSION,IN_INTER,FUN_FMAP_DEF,combinTheory.APPLY_UPDATE_THM]
+      >> rw [FAPPLY_FUPDATE_THM])
+QED
 
 Theorem equiv2 :
-  ∀E E' t inE outE stateIn stateOut.
-    Supports E iter_arithprog ∧
-    inE = strmIndex (input_of iter_arithprog E) t ∧
-    stateIn = strmIndex (state_of iter_arithprog E) t
-    (stateOut,outE) = stateStep iter_arithprog (inE,stateIn)
-    E' = strmStep E iter_arithprog t ∧
+  ∀E E't t inputs.
+    Supports E itprog ∧
+    isInit_Stream (E ' "isInit") ∧
+    E't = strmIndex (strmSteps E itprog t) t ∧
+    inputs = input_of itprog E
     ⇒
-      (strmIndex (state_of iter_arithprog E') t,
-       strmIndex (output_of iter_arithprog E') t)
+      (state_of itprog E't, output_of itprog E't)
       =
-     (stateOut,outE)
+      stateSteps inputs initState itprog t
 Proof
-  EVAL_TAC >> rw []
+  simp[]
+  >> Induct_on ‘t’
+  >- (expand_Supports
+      >> rw [stateSteps_def, strmSteps_def,stateStep_def,input_of_def,
+             itprog_inports, itprog_var_defs,itprog_out_defs]
+      >> rw [strmIndex_DRESTRICT,lem]
+      >> rw [FUPDATE_LIST_THM,FUNION_FUPDATE_1]
+      >> CONV_TAC (RAND_CONV EVAL)
+      >> CONV_TAC (PATH_CONV "rlr" finite_mapLib.fupdate_NORMALISE_CONV)
+      >> rw [DRESTRICT_FUPDATE]
+      >> rw [strmStep_def,itprog_inports,itprog_var_defs,itprog_out_defs]
+      >> rw[fmap_EXT]
+      >> CONV_TAC (RATOR_CONV EVAL)
+      >- (rw [DRESTRICT_DEF,EXTENSION,IN_INTER] >> metis_tac[])
+      >- (rw [DRESTRICT_DEF,FUN_FMAP_DEF] >> EVAL_TAC >> metis_tac[])
+      >- (rw [DRESTRICT_DEF,EXTENSION,IN_INTER] >> metis_tac[])
+      >- (rw [DRESTRICT_DEF,FUN_FMAP_DEF] >> EVAL_TAC >> metis_tac[])
+     )
+
+  >- (rpt strip_tac
+      >> ‘Supports (strmSteps E itprog t) itprog’ by metis_tac [Supports_strmSteps]
+      >> ‘isInit_Stream (strmSteps E itprog t ' "isInit")’
+            by (‘Wellformed itprog’ by (EVAL_TAC >> simp[]) >>
+                ‘MEM "isInit" itprog.inports’ by EVAL_TAC >>
+                metis_tac [isInit_Stable])
+      >> ‘stateSteps (input_of itprog E) initState itprog t
+          =
+         (state_of itprog (strmIndex (strmSteps E itprog t) t),
+          output_of itprog (strmIndex (strmSteps E itprog t) t))’ by metis_tac[]
+      >> WEAKEN_TAC is_forall
+      >> rw [stateSteps_def]
+      >> rw [Once EQ_SYM_EQ]
+      >> irule equiv2_step
+      >> rw[]
+      >> qexists_tac ‘strmSteps E itprog t’
+      >> rw[]
+         >- rw [strmSteps_def]
+         >- (‘Wellformed itprog’ by (EVAL_TAC >> rw[]) >> metis_tac[input_of_stable])
+     )
 QED
-*)
 
 (*---------------------------------------------------------------------------*)
-(* "pre-CakeML" logic function version of iter_arithprog. Note that variable *)
-(* in2 is a parameter when it doesn't strictly have to be.                   *)
+(* "pre-CakeML" logic function version of itprog. Note that variable in2 is  *)
+(* a parameter when it doesn't strictly have to be.                          *)
 (*---------------------------------------------------------------------------*)
 
 Definition aprogFn_def :
@@ -234,23 +362,9 @@ Definition aprogFn_def :
 End
 
 (*---------------------------------------------------------------------------*)
-(* Now interpret iter_arithprog in a setting where the environments are      *)
-(* string |-> value maps, instead of the string |-> value stream maps being  *)
-(* used in agreeScript.                                                      *)
+(* Show that aprogFn is equal to stateStep, i.e. that the logic function is  *)
+(* equal to the valEnv transformer.                                          *)
 (*---------------------------------------------------------------------------*)
-
-(*---------------------------------------------------------------------------*)
-(* Lemma that state_ap = out_ap. Not used.                                   *)
-(*---------------------------------------------------------------------------*)
-
-Theorem out_eq_ap :
-  ∀inE stateIn stateOut outE.
-      (stateOut,outE) = stateStep iter_arithprog (inE,stateIn)
-  ⇒
-  (outE ' "out") = (stateOut ' "ap")
-Proof
-  EVAL_TAC >> rw[] >> rpt(pop_assum mp_tac) >> rw[] >> EVAL_TAC
-QED
 
 Theorem equiv3 :
   ∀input isInit N ap in2 in1.
@@ -260,7 +374,7 @@ Theorem equiv3 :
                         ("ap",   BoolValue ap);
                         ("in2",  IntValue in2);
                         ("in1",  IntValue in1)];
-         (stateOut,outE) = stateStep iter_arithprog (inE,stateIn) ;
+         (stateOut,outE) = stateStep itprog (inE,stateIn) ;
          state_N     = int_of(stateOut ' "N");
          state_ap    = bool_of(stateOut ' "ap");
          state_in2   = int_of(stateOut ' "in2");
@@ -281,5 +395,17 @@ Proof
 QED
 
 
+(*---------------------------------------------------------------------------*)
+(* Lemma that state_ap = out_ap. Not used.                                   *)
+(*---------------------------------------------------------------------------*)
+
+Theorem out_eq_ap :
+  ∀inE stateIn stateOut outE.
+      (stateOut,outE) = stateStep itprog (inE,stateIn)
+  ⇒
+  (outE ' "out") = (stateOut ' "ap")
+Proof
+  EVAL_TAC >> rw[] >> rpt(pop_assum mp_tac) >> rw[] >> EVAL_TAC
+QED
 
 val _ = export_theory();
